Notation Update

theories/CCSInstance.v
@@ -26,11 +26,33 @@
 Require Import Coq.Program.Equality Coq.Strings.String.
 From stdpp Require Import base countable finite gmap list gmultiset strings.
 Require Import Relations.
-From Must Require Import TransitionSystems Must Completeness.
-
 Require Import Coq.Wellfounded.Inverse_Image.
 
-Definition name := string.
+
+(* ChannelType est le type des canaux, par exemple des chaînes de caractères*)
+(* ValueType est le type des données transmises, par exemple des entiers, des chaînes de caractères, des programmes (?) *)
+Inductive ExtAct (Channel: Type) :=
+| ActIn : Channel -> ExtAct Channel
+| ActOut : Channel -> ExtAct Channel
+.
+
+Arguments ActIn {_} _ .
+Arguments ActOut {_} _ .
+
+Inductive Act (Channel : Type) :=
+| ActExt (μ: ExtAct Channel)
+| τ
+.
+Arguments ActExt {_} _.
+Arguments τ {_} .
+
+
+Coercion ActExt : ExtAct >-> Act.
+
+Context (Channel Value : Type).
+(*Exemple : Definition Channel := string.*)
+(*Exemple : Definition Value := nat.*)
+
 
 (* Definition of processes*)
 Inductive proc : Type :=
@@ -48,127 +70,112 @@ with gproc : Type :=
 | gpr_success : gproc
 (* The Process that does nothing*)
 | gpr_nil : gproc
-(*An input is a name of a channel followed by a process*)
-| gpr_input : name -> proc -> gproc
-(*An output is a name of a channel followed by a process*)
-| gpr_output : name -> proc -> gproc
+(*An input is a Channel of a channel followed by a process*)
+| gpr_input : Channel -> proc -> gproc
+(*An output is a Channel of a channel followed by a process*)
+| gpr_output : Channel -> proc -> gproc
 (*A tau action : does nothing *)
 | gpr_tau : proc -> gproc
 (* To choose between two processes*)
 | gpr_choice : gproc -> gproc -> gproc
 .
 
-(* decision procedure to equal processes*)
-Fixpoint proc_dec (x y : proc) : { x = y } + { x <> y }
-with gproc_dec (x y : gproc) : { x = y } + { x <> y }.
-Proof.
-  decide equality; destruct (decide (n = n0)); eauto.
-  decide equality; destruct (decide (n = n0)); eauto.
-Qed.
+Coercion pr_var : nat >-> proc.
+Coercion g : gproc >-> proc.
 
-#[global] Instance proc_eq_decision_instance : EqDecision proc.
-Proof. by exact proc_dec. Defined.
-
-
-Notation pr_success := (g gpr_success).
-Notation θ := (g gpr_nil).
-Notation pr_input a p := (g (gpr_input a p)).
-Notation pr_output a p := (g (gpr_output a p)).
-Notation pr_tau p := (g (gpr_tau p)).
-Notation pr_choice p q := (g (gpr_choice p q)).
-
-(*Some notation to simplify the view of the code*)
-Infix "∥" := pr_par (at level 50).
-Infix "˖" := pr_choice (at level 50).
-Infix "?" := gpr_input (at level 50).
-Infix "!" := gpr_output (at level 50).
+Notation "①" := (gpr_success).
+Notation "⓪" := (gpr_nil).
+Notation "'rec' x '•' p" := (pr_rec x p) (at level 50).
+Notation "P + Q" := (gpr_choice P Q).
+Notation "P ‖ Q" := (pr_par P Q) (at level 50).
+Notation "c ! • P" := (gpr_output c P) (at level 50).
+Notation "c ? • P" := (gpr_input c P) (at level 50).
+Notation "'t' • P" := (gpr_tau P) (at level 50).
 
 
 (*Definition for the size of a term : proc, to do induction on it in the future*)
 Fixpoint size (p : proc) :=
   match p with
-  | pr_par p q  => S (size p + size q)
+  | p ‖ q  => S (size p + size q)
   | pr_var _ => 1
-  | pr_rec x p => S (size p)
+  | rec x • p => S (size p)
   | g p => gsize p
   end
 
 with gsize p :=
   match p with
-  | gpr_success => 1
-  | gpr_nil => 0
-  | gpr_input a p => S (size p)
-  | gpr_output a p => S (size p)
-  | gpr_tau p => S (size p)
-  | gpr_choice p q => S (gsize p + gsize q)
+  | ① => 1
+  | ⓪ => 0
+  | c ! • p => S (size p)
+  | c ? • p => S (size p)
+  | t • p => S (size p)
+  | p + q => S (gsize p + gsize q)
   end.
 
 
 (* Substitution, usefull for Recursion def and Context definition (for congruence) *)
 Fixpoint pr_subst id p q :=
   match p with
-  | pr_par p1 p2 => pr_par (pr_subst id p1 q) (pr_subst id p2 q)
+  | p1 ‖ p2 => pr_par (pr_subst id p1 q) (pr_subst id p2 q)
   | pr_var id' => if decide (id = id') then q else p
-  | pr_rec id' p' =>
-    if decide (id = id') then p else pr_rec id' (pr_subst id p' q)
+  | rec id' • p' =>
+    if decide (id = id') then p else rec id' • (pr_subst id p' q)
   | g gp => g (gpr_subst id gp q)
 end
 
 with gpr_subst id p q {struct p} := match p with
-| gpr_success => p
-| gpr_nil => p
-| gpr_input a p =>
-    gpr_input a (pr_subst id p q)
-
-| gpr_output a p =>
-    gpr_output a (pr_subst id p q)
-
-| gpr_tau p =>
-    gpr_tau (pr_subst id p q)
-| gpr_choice p1 p2 =>
-    gpr_choice (gpr_subst id p1 q) (gpr_subst id p2 q)
+| ① => p
+| ⓪ => p
+| c ! • p =>
+    c ! • (pr_subst id p q)
+| c ? • p =>
+    c ? • (pr_subst id p q)
+| t • p =>
+    t • (pr_subst id p q)
+| p1 + p2 =>
+    (gpr_subst id p1 q) + (gpr_subst id p2 q)
 end.
 
 
 (* The Labelled Transition System (LTS-transition) *)
-Inductive lts : proc -> Act name -> proc -> Prop :=
+Inductive lts : proc -> Act Channel -> proc -> Prop :=
 (*The Input and the Output*)
-| lts_input : forall {a t},
-    lts (pr_input a t) (ActExt (ActIn a)) t
-| lts_output : forall {a t},
-    lts (pr_output a t) (ActExt (ActOut a)) t
+| lts_input : forall {c p},
+    lts (c ? • p) (ActExt (ActIn c)) p
+| lts_output : forall {c p},
+    lts (c ! • p) (ActExt (ActOut c)) p
 
 (*The actions Tau*)
-| lts_tau : forall {t},
-    lts (pr_tau t) τ t
+| lts_tau : forall {p},
+    lts (t • p) τ p
 | lts_rec : forall {x p},
-    lts (pr_rec x p) τ (pr_subst x p (pr_rec x p))
+    lts (rec x • p) τ (pr_subst x p (rec x • p))
 
-(* Communication of a channel output and input that have the same name*)
+(* Communication of a channel output and input that have the same Channel*)
 | lts_comL : forall {a p1 p2 q1 q2},
     lts p1 (ActExt (ActOut a)) p2 ->
     lts q1 (ActExt (ActIn a)) q2 ->
-    lts (pr_par p1 q1) τ (pr_par p2 q2)
+    lts (p1 ‖ q1) τ (p2 ‖ q2)
 | lts_comR : forall {a p1 p2 q1 q2},
     lts p1 (ActExt (ActOut a)) p2 ->
     lts q1 (ActExt (ActIn a)) q2 ->
-    lts (pr_par q1 p1) τ (pr_par q2 p2)
+    lts (q1 ‖ p1) τ (q2 ‖ p2)
 
 (*The decoration for the transition system...*)
 (*...for the parallele*)
 | lts_parL : forall {α p1 p2 q},
     lts p1 α p2 ->
-    lts (pr_par p1 q) α (pr_par p2 q)
+    lts (p1 ‖ q) α (p2 ‖ q)
 | lts_parR : forall {α p q1 q2},
     lts q1 α q2 ->
-    lts (pr_par p q1) α (pr_par p q2)
+    lts (p ‖ q1) α (p ‖ q2)
 (*...for the sum*)
 | lts_choiceL : forall {p1 p2 q α},
     lts (g p1) α q ->
-    lts (pr_choice p1 p2) α q
+    lts (p1 + p2) α q
 | lts_choiceR : forall {p1 p2 q α},
     lts (g p2) α q ->
-    lts (pr_choice p1 p2) α q
+    lts (p1 + p2) α q
 .
 
 
@@ -181,50 +188,51 @@ Inductive cgr_step : proc -> proc -> Prop :=
 | cgr_refl_step : forall p, p ≡ p
 
 (* Rules for the Parallèle *)
-| cgr_par_nil_step : forall p,
-    p ∥ θ ≡ p
+| cgr_par_nil_step : forall p, 
+    p ‖ ⓪ ≡ p
 | cgr_par_nil_rev_step : forall p,
-    p ≡ p ∥ θ
+    p ≡ p ‖ ⓪
 | cgr_par_com_step : forall p q,
-    p ∥ q ≡ q ∥ p
+    p ‖ q ≡ q ‖ p
 | cgr_par_assoc_step : forall p q r,
-    (p ∥ q) ∥ r ≡ p ∥(q ∥r)
+    (p ‖ q) ‖ r ≡ p ‖ (q ‖ r)
 | cgr_par_assoc_rev_step : forall p q r,
-    p ∥(q ∥ r) ≡ (p ∥ q) ∥ r
+    p ‖ (q  ‖ r) ≡ (p ‖ q) ‖ r
 
 (* Rules for the Summation *)
 | cgr_choice_nil_step : forall p,
-    p ˖ gpr_nil ≡ (g p)
+    cgr_step (p + ⓪) p
 | cgr_choice_nil_rev_step : forall p,
-    (g p) ≡ p ˖ gpr_nil
+    cgr_step (g p) (p + ⓪)
 | cgr_choice_com_step : forall p q,
-    p ˖ q ≡ q ˖ p
+    cgr_step (p + q) (q + p)
 | cgr_choice_assoc_step : forall p q r,
-    (gpr_choice p  q) ˖ r ≡ p ˖ (gpr_choice q r)
+    cgr_step ((p + q) + r) (p + (q + r))
 | cgr_choice_assoc_rev_step : forall p q r,
-    p ˖ (gpr_choice q r) ≡ (gpr_choice p q) ˖ r
+    cgr_step (p + (q + r)) ((p + q) + r)
 
 (*The reduction is given to certain terms...*)
 | cgr_recursion_step : forall x p q,
-    cgr_step p q -> (pr_rec x p) ≡ (pr_rec x q)
+    cgr_step p q -> (rec x • p) ≡ (rec x • q)
 | cgr_tau_step : forall p q,
     cgr_step p q ->
-    (pr_tau p) ≡ (pr_tau q)
-| cgr_input_step : forall a p q,
+    cgr_step (t • p) (t • q)
+| cgr_input_step : forall c p q,
     cgr_step p q ->
-    (pr_input a p) ≡ (pr_input a q)
-| cgr_output_step : forall a p q,
+    cgr_step (c ? • p) (c ? • q)
+| cgr_output_step : forall c p q,
     cgr_step p q ->
-    (pr_output a p) ≡ (pr_output a q)
+    cgr_step (c ! • p) (c ! • q)
 | cgr_par_step : forall p q r,
-    cgr_step p q->
-    p ∥ r ≡ q ∥ r
+    cgr_step p q ->
+    p ‖ r ≡ q ‖ r
 
-(*...and sums (only for gards (by sanity))*)
+(*...and sums (only for guards (by sanity))*)
 | cgr_choice_step : forall p1 q1 p2,
     cgr_step (g p1) (g q1) -> 
-    p1 ˖ p2 ≡ q1 ˖ p2
+    cgr_step (p1 + p2) (q1 + p2)
 .
+
 
 
 #[global] Hint Constructors cgr_step:cgr_step_structure.
@@ -264,87 +272,87 @@ Proof. repeat split.
 Qed.
 
 (*the relation ≡* respects all the rules that ≡ respected*)
-Lemma cgr_par_nil : forall p, p ∥ θ ≡* p.
+Lemma cgr_par_nil : forall p, p ‖ ⓪ ≡* p.
 Proof.
 constructor.
 apply cgr_par_nil_step.
 Qed.
-Lemma cgr_par_nil_rev : forall p, p ≡* p ∥ θ.
+Lemma cgr_par_nil_rev : forall p, p ≡* p ‖ ⓪.
 Proof.
 constructor.
 apply cgr_par_nil_rev_step.
 Qed.
-Lemma cgr_par_com : forall p q, p ∥ q ≡* q ∥ p.
+Lemma cgr_par_com : forall p q, p ‖ q ≡* q ‖ p.
 Proof.
 constructor.
 apply cgr_par_com_step.
 Qed.
-Lemma cgr_par_assoc : forall p q r, (p ∥ q) ∥ r ≡* p ∥(q ∥r).
+Lemma cgr_par_assoc : forall p q r, (p ‖ q) ‖ r ≡* p ‖(q ‖r).
 Proof.
 constructor.
 apply cgr_par_assoc_step.
 Qed.
-Lemma cgr_par_assoc_rev : forall p q r, p ∥(q ∥ r) ≡* (p ∥ q) ∥ r.
+Lemma cgr_par_assoc_rev : forall p q r, p ‖(q ‖ r) ≡* (p ‖ q) ‖ r.
 Proof.
 constructor.
 apply cgr_par_assoc_rev_step.
 Qed.
-Lemma cgr_choice_nil : forall p, p ˖ gpr_nil ≡* (g p).
+Lemma cgr_choice_nil : forall p, p + ⓪ ≡* p.
 Proof.
 constructor.
 apply cgr_choice_nil_step.
 Qed.
-Lemma cgr_choice_nil_rev : forall p, (g p) ≡* p ˖ gpr_nil.
+Lemma cgr_choice_nil_rev : forall p, g p ≡* p + ⓪.
 Proof.
 constructor.
 apply cgr_choice_nil_rev_step.
 Qed.
-Lemma cgr_choice_com : forall p q, p ˖ q ≡* q ˖ p.
+Lemma cgr_choice_com : forall p q, p + q ≡* q + p.
 Proof.
 constructor.
 apply cgr_choice_com_step.
 Qed.
-Lemma cgr_choice_assoc : forall p q r, (gpr_choice p  q) ˖ r ≡* p ˖ (gpr_choice q r).
+Lemma cgr_choice_assoc : forall p q r, (p + q) + r ≡* p + (q + r).
 Proof.
 constructor.
 apply cgr_choice_assoc_step.
 Qed.
-Lemma cgr_choice_assoc_rev : forall p q r, p ˖ (gpr_choice q r) ≡* (gpr_choice p q) ˖ r.
+Lemma cgr_choice_assoc_rev : forall p q r, p + (q + r) ≡* (p + q) + r.
 Proof.
 constructor.
 apply cgr_choice_assoc_rev_step.
 Qed.
-Lemma cgr_recursion : forall x p q, p ≡* q -> (pr_rec x p) ≡* (pr_rec x q).
+Lemma cgr_recursion : forall x p q, p ≡* q -> (rec x • p) ≡* (rec x • q).
 Proof.
 intros. dependent induction H. 
 constructor. 
 apply cgr_recursion_step. exact H. eauto with cgr_eq.
 Qed.
-Lemma cgr_tau : forall p q, p ≡* q -> (pr_tau p) ≡* (pr_tau q).
+Lemma cgr_tau : forall p q, p ≡* q -> (t • p) ≡* (t • q).
 Proof.
 intros. dependent induction H. 
 constructor. 
 apply cgr_tau_step. exact H. eauto with cgr_eq.
 Qed. 
-Lemma cgr_input : forall a p q, p ≡* q -> (pr_input a p) ≡* (pr_input a q).
+Lemma cgr_input : forall c p q, p ≡* q -> (c ? • p) ≡* (c ? • q).
 Proof.
 intros. dependent induction H. 
 constructor.
 apply cgr_input_step. exact H. eauto with cgr_eq.
 Qed. 
-Lemma cgr_output : forall a p q, p ≡* q -> (pr_output a p) ≡* (pr_output a q).
+Lemma cgr_output : forall c p q, p ≡* q -> (c ! • p) ≡* (c ! • q).
 Proof.
 intros. dependent induction H. 
 constructor.
 apply cgr_output_step. exact H. eauto with cgr_eq.
 Qed.
-Lemma cgr_par : forall p q r, p ≡* q-> p ∥ r ≡* q ∥ r.
+Lemma cgr_par : forall p q r, p ≡* q-> p ‖ r ≡* q ‖ r.
 Proof.
 intros. dependent induction H. 
 constructor.
 apply cgr_par_step. exact H. eauto with cgr_eq.
 Qed.
-Lemma cgr_choice : forall p1 q1 p2, (g p1) ≡* (g q1) ->  p1 ˖ p2 ≡* q1 ˖ p2.
+Lemma cgr_choice : forall p1 q1 p2, (g p1) ≡* (g q1) ->  p1 + p2 ≡* q1 + p2.
 Proof.
 intros. dependent induction H. 
   - constructor. apply cgr_choice_step. exact H.
@@ -353,24 +361,24 @@ Admitted.
 
 
 (* The sum of guards respects ≡* *)
-Lemma cgr_fullchoice : forall M1 M2 M3 M4, g M1 ≡* g M2 -> g M3 ≡* g M4 -> M1 ˖ M3 ≡* M2 ˖ M4.
+Lemma cgr_fullchoice : forall M1 M2 M3 M4, g M1 ≡* g M2 -> g M3 ≡* g M4 -> M1 + M3 ≡* M2 + M4.
 Proof.
 intros.
-apply transitivity with (M2 ˖ M3). apply cgr_choice. exact H. apply transitivity with (M3 ˖ M2).
-apply cgr_choice_com. apply transitivity with (M4 ˖ M2). apply cgr_choice. exact H0. apply cgr_choice_com.
+apply transitivity with (g (M2 + M3)). apply cgr_choice. exact H. apply transitivity with (g (M3 + M2)).
+apply cgr_choice_com. apply transitivity with (g (M4 + M2)). apply cgr_choice. exact H0. apply cgr_choice_com.
 Qed.
 (* The parallele of process respects ≡* *)
-Lemma cgr_fullpar : forall M1 M2 M3 M4, M1 ≡* M2 -> M3 ≡* M4 -> M1 ∥ M3 ≡* M2 ∥ M4.
+Lemma cgr_fullpar : forall M1 M2 M3 M4, M1 ≡* M2 -> M3 ≡* M4 -> M1 ‖ M3 ≡* M2 ‖ M4.
 Proof.
 intros.
-apply transitivity with (M2 ∥ M3). apply cgr_par. exact H. apply transitivity with (M3 ∥ M2).
-apply cgr_par_com. apply transitivity with (M4 ∥ M2). apply cgr_par. exact H0. apply cgr_par_com.
+apply transitivity with (M2 ‖ M3). apply cgr_par. exact H. apply transitivity with (M3 ‖ M2).
+apply cgr_par_com. apply transitivity with (M4 ‖ M2). apply cgr_par. exact H0. apply cgr_par_com.
 Qed.
 
-(* Decision procedure for the name of channel *)
-Definition name_eq_dec : forall (x y : name), { x = y } + { x <> y } := string_dec.
+(*(* Decision procedure for the Channel of channel *)
+Definition Channel_eq_dec : forall (x y : Channel), { x = y } + { x <> y } := string_dec.
 
-#[global] Instance name_eqdecision : EqDecision name. by exact name_eq_dec. Defined.
+#[global] Instance Channel_eqdecision : EqDecision Channel. by exact Channel_eq_dec. Defined.*)
 
 
 #[global] Hint Resolve cgr_par_nil cgr_par_nil_rev cgr_par_nil_rev cgr_par_com cgr_par_assoc 
@@ -382,20 +390,20 @@ cgr_refl cgr_symm cgr_trans:cgr.
 (* State Transition System (STS-reduction) *)
 Inductive sts : proc -> proc -> Prop :=
 (*The axiomes*)
-(* Communication of channels output and input that have the same name *)
-| sts_com : forall {μ p1 m1 p2 m2},
-    sts (pr_par(pr_choice (gpr_output μ p1) (m1)) (pr_choice (gpr_input μ p2) (m2))) (pr_par p1 p2)
+(* Communication of channels output and input that have the same Channel *)
+| sts_com : forall {c p1 g1 p2 g2},
+    sts (((c ! • p1) + g1) ‖ ((c ? • p2) + g2)) (p1 ‖ p2)
 (* Nothing more , something less *)
-| sts_tau : forall {t m},
-    sts (pr_choice (gpr_tau t) m) t
+| sts_tau : forall {p g},
+    sts ((t • p) + g) p
 (* Resursion *)
 | sts_rec : forall {x p},
-    sts (pr_rec x p) (pr_subst x p (pr_rec x p))
+    sts (rec x • p) (pr_subst x p (rec x • p))
 
 (* The left parallele respect the Reduction *)
 | sts_par : forall {p1 p2 q},
     sts p1 p2 ->
-    sts (pr_par p1 q) (pr_par p2 q)
+    sts (p1 ‖ q) (p2 ‖ q)
 
 (*The Congruence respects the Reduction *)
 | sts_cong : forall {p1 p2 q2 q1},
@@ -407,26 +415,26 @@ Infix "➙" := sts (at level 50).
 
 (* For the (STS-reduction), the reductible terms and reducted terms are pretty all the same, up to ≡* *)
 Lemma ReductionShape : forall P Q, P ➙ Q ->
-((exists x P1 P2 M1 M2 S, ((P ≡* (((x ! P1) ˖ M1) ∥ ((x ? P2) ˖ M2)) ∥ S)) /\ (Q ≡*((P1 ∥ P2) ∥ S)))
-\/ (exists P1 M1 S, (P ≡* (((gpr_tau P1) ˖ M1) ∥ S)) /\ (Q ≡* (P1 ∥ S)))
-\/ (exists n P1 S, (P ≡* ((pr_rec n P1) ∥ S)) /\ (Q ≡* (pr_subst n P1 (pr_rec n P1) ∥ S)))).
+((exists x P1 P2 M1 M2 S, ((P ≡* (((x ! • P1) + M1) ‖ ((x ? • P2) + M2)) ‖ S)) /\ (Q ≡*((P1 ‖ P2) ‖ S)))
+\/ (exists P1 M1 S, (P ≡* (((t • P1) + M1) ‖ S)) /\ (Q ≡* (P1 ‖ S)))
+\/ (exists n P1 S, (P ≡* ((rec n • P1) ‖ S)) /\ (Q ≡* (pr_subst n P1 (rec n • P1) ‖ S)))).
 Proof.
 intros P Q Transition.
 induction Transition.
-  - left. exists μ. exists p1. exists p2. exists m1. exists m2. exists (g gpr_nil). split; apply cgr_par_nil_rev.
-  - right. left. exists t. exists m. exists θ. split; apply cgr_par_nil_rev.
-  - right. right. exists x. exists p. exists θ. split; apply cgr_par_nil_rev.
+  - left. exists c. exists p1. exists p2. exists g1. exists g2. exists ⓪. split; apply cgr_par_nil_rev.
+  - right. left. exists p. exists g0. exists ⓪. split; apply cgr_par_nil_rev.
+  - right. right. exists x. exists p. exists ⓪. split; apply cgr_par_nil_rev.
   - destruct IHTransition as [IH|[IH|IH]]; [ left | right; left | right; right]; decompose record IH.
-    * exists x. exists x0. exists x1. exists x2. exists x3. exists (x4 ∥ q). split.
-        ** apply transitivity with (((((x ! x0) ˖ x2) ∥ ((x ? x1) ˖ x3)) ∥ x4) ∥ q). apply cgr_par. exact H. apply cgr_par_assoc.
-        ** apply transitivity with (((x0 ∥ x1) ∥ x4) ∥ q). apply cgr_par. exact H1.  apply cgr_par_assoc.
-    * exists x. exists x0. exists (x1 ∥ q). split.
-        ** apply transitivity with (((gpr_tau x ˖ x0) ∥ x1) ∥ q). apply cgr_par. exact H0.
+    * exists x. exists x0. exists x1. exists x2. exists x3. exists (x4 ‖ q). split.
+        ** apply transitivity with (((((x ! • x0) + x2) ‖ ((x ? • x1) + x3)) ‖ x4) ‖ q). apply cgr_par. exact H. apply cgr_par_assoc.
+        ** apply transitivity with (((x0 ‖ x1) ‖ x4) ‖ q). apply cgr_par. exact H1.  apply cgr_par_assoc.
+    * exists x. exists x0. exists (x1 ‖ q). split.
+        ** apply transitivity with (((t • x + x0) ‖ x1) ‖ q). apply cgr_par. exact H0.
         apply cgr_par_assoc.
-        ** apply transitivity with (x ∥(x1) ∥ q). apply cgr_par. exact H1. apply cgr_par_assoc.
-    * exists x. exists x0. exists (x1 ∥ q). split. 
-        ** apply transitivity with ((pr_rec x x0 ∥ x1) ∥ q). apply cgr_par. exact H0. apply cgr_par_assoc.
-        ** apply transitivity with ((pr_subst x x0 (pr_rec x x0) ∥ x1) ∥ q). apply cgr_par. exact H1. apply cgr_par_assoc.
+        ** apply transitivity with (x ‖(x1) ‖ q). apply cgr_par. exact H1. apply cgr_par_assoc.
+    * exists x. exists x0. exists (x1 ‖ q). split. 
+        ** apply transitivity with ((rec x • x0 ‖ x1) ‖ q). apply cgr_par. exact H0. apply cgr_par_assoc.
+        ** apply transitivity with ((pr_subst x x0 (rec x • x0) ‖ x1) ‖ q). apply cgr_par. exact H1. apply cgr_par_assoc.
   - destruct IHTransition as [IH|[IH|IH]]; [ left | right; left | right; right];  decompose record IH.
     * exists x. exists x0. exists x1. exists x2. exists x3. exists x4. split. apply cgr_trans with p2. exact H. exact H1.
       apply cgr_trans with q2. apply cgr_symm. exact H0. exact H3.
@@ -439,78 +447,78 @@ Qed.
 
 (* For the (LTS-transition), the transitable terms and transitted terms, that performs a INPUT,
 are pretty all the same, up to ≡* *)
-Lemma TransitionShapeForInput : forall P V x, (lts P (ActExt (ActIn x)) V -> 
-(exists Q M R, ((P ≡* ((x ? Q) ˖ M) ∥ R)) /\ (V ≡* (Q ∥ R)) /\ ((exists L,P = (g L)) -> R = θ))).
+Lemma TransitionShapeForInput : forall P V x, (lts P (ActIn x) V -> 
+(exists Q M R, ((P ≡* ((x ? • Q) + M) ‖ R)) /\ (V ≡* (Q ‖ R)) /\ ((exists L,P = (g L)) -> R = ⓪))).
 Proof.
 intros P V x Transition.
  dependent induction Transition.
-- exists t. exists gpr_nil. exists θ. split ; try split.
-  * apply cgr_trans with ((x ? t) ˖ gpr_nil). apply cgr_trans with (g (x ? t)). apply cgr_refl. apply cgr_choice_nil_rev. apply cgr_par_nil_rev.
+- exists p. exists ⓪. exists ⓪. split ; try split.
+  * apply cgr_trans with ((x ? • p) + ⓪). apply cgr_trans with (x ? • p). apply cgr_refl. apply cgr_choice_nil_rev. apply cgr_par_nil_rev.
   * apply cgr_par_nil_rev.
   * reflexivity.
-- destruct (IHTransition x). reflexivity. decompose record H. exists x0. exists x1. exists (x2 ∥ q). split; try split.
-  * apply cgr_trans with ((((x ? x0) ˖ x1) ∥ x2) ∥ q). apply cgr_par. exact H0. apply cgr_par_assoc.
-  * apply cgr_trans with ((x0 ∥ x2) ∥ q). apply cgr_par. exact H1. apply cgr_par_assoc.
+- destruct (IHTransition x). reflexivity. decompose record H. exists x0. exists x1. exists (x2 ‖ q). split; try split.
+  * apply cgr_trans with ((((x ? • x0) + x1) ‖ x2) ‖ q). apply cgr_par. exact H0. apply cgr_par_assoc.
+  * apply cgr_trans with ((x0 ‖ x2) ‖ q). apply cgr_par. exact H1. apply cgr_par_assoc.
   * intros. inversion H2. inversion H4.
-- destruct (IHTransition x). reflexivity. decompose record H. exists x0. exists x1. exists (x2 ∥ p). split; try split.
-  * apply cgr_trans with ((((x ? x0) ˖ x1) ∥ x2) ∥ p). apply cgr_trans with (q1 ∥ p). apply cgr_par_com. apply cgr_par. exact H0. apply cgr_par_assoc.
-  * apply cgr_trans with ((x0 ∥ x2) ∥ p). apply cgr_trans with (q2 ∥ p). apply cgr_par_com. apply cgr_par. exact H1. apply cgr_par_assoc.
+- destruct (IHTransition x). reflexivity. decompose record H. exists x0. exists x1. exists (x2 ‖ p). split; try split.
+  * apply cgr_trans with ((((x ? • x0) + x1) ‖ x2) ‖ p). apply cgr_trans with (q1 ‖ p). apply cgr_par_com. apply cgr_par. exact H0. apply cgr_par_assoc.
+  * apply cgr_trans with ((x0 ‖ x2) ‖ p). apply cgr_trans with (q2 ‖ p). apply cgr_par_com. apply cgr_par. exact H1. apply cgr_par_assoc.
   * intros. inversion H2. inversion H4.
-- destruct (IHTransition x). reflexivity. decompose record H. exists x0. exists (gpr_choice x1 p2). exists θ. split ; try split.
-  * apply cgr_trans with ((x ? x0) ˖ gpr_choice x1 p2). apply cgr_trans with ((gpr_choice (x ? x0) x1) ˖ p2).
-    apply cgr_choice. assert (x2 = θ). apply H3. exists p1. reflexivity. rewrite H2 in H0. apply transitivity with (((x ? x0) ˖ x1) ∥ θ).
+- destruct (IHTransition x). reflexivity. decompose record H. exists x0. exists (x1 + p2). exists ⓪. split ; try split.
+  * apply cgr_trans with ((x ? • x0) + (x1 + p2)). apply cgr_trans with (((x ? • x0) + x1) + p2).
+    apply cgr_choice. assert (x2 = ⓪). apply H3. exists p1. reflexivity. rewrite H2 in H0. apply transitivity with (((x ? • x0) + x1) ‖ ⓪).
     exact H0. apply cgr_par_nil. apply cgr_choice_assoc. apply cgr_par_nil_rev.
-  * assert (x2 = θ). apply H3. exists p1. reflexivity. rewrite H2 in H1. exact H1.
+  * assert (x2 = ⓪). apply H3. exists p1. reflexivity. rewrite H2 in H1. exact H1.
   * reflexivity.
-- destruct (IHTransition x). reflexivity. decompose record H. exists x0. exists (gpr_choice x1 p1). exists θ. split; try split.
-  * apply cgr_trans with ((x ? x0) ˖ gpr_choice x1 p1). apply cgr_trans with ((gpr_choice (x ? x0) x1) ˖ p1).
-    apply cgr_trans with (p2 ˖ p1). apply cgr_choice_com. apply cgr_choice. assert (x2 = θ). apply H3. exists p2. reflexivity.
-    apply cgr_trans with (((x ? x0) ˖ x1) ∥ x2). exact H0. rewrite H2. apply cgr_par_nil. apply cgr_choice_assoc. apply cgr_par_nil_rev.
-  * assert (x2 = θ). apply H3. exists p2. reflexivity. rewrite <-H2. exact H1.
+- destruct (IHTransition x). reflexivity. decompose record H. exists x0. exists (x1 + p1). exists ⓪. split; try split.
+  * apply cgr_trans with ((x ? • x0) + (x1 + p1)). apply cgr_trans with (((x ? • x0) + x1) + p1).
+    apply cgr_trans with (p2 + p1). apply cgr_choice_com. apply cgr_choice. assert (x2 = ⓪). apply H3. exists p2. reflexivity.
+    apply cgr_trans with (((x ? • x0) + x1) ‖ x2). exact H0. rewrite H2. apply cgr_par_nil. apply cgr_choice_assoc. apply cgr_par_nil_rev.
+  * assert (x2 = ⓪). apply H3. exists p2. reflexivity. rewrite <-H2. exact H1.
   * reflexivity.
 Qed.
 
 (* For the (LTS-transition), the transitable terms and transitted terms, that performs a OUPUT,
 are pretty all the same, up to ≡* *)
-Lemma TransitionShapeForOutput : forall P V x, (lts P (ActExt (ActOut x)) V -> 
-(exists Q M R, ((P ≡* ((x! Q) ˖ M) ∥ R)) /\ (V ≡* (Q ∥ R)) /\ ((exists L,P = (g L)) -> R = θ))).
+Lemma TransitionShapeForOutput : forall P V x, (lts P (ActOut x) V -> 
+(exists Q M R, ((P ≡* ((x ! • Q) + M) ‖ R)) /\ (V ≡* (Q ‖ R)) /\ ((exists L,P = (g L)) -> R = ⓪))).
 Proof.
 intros P V x Transition.
  dependent induction Transition.
-- exists t. exists gpr_nil. exists θ. split ; try split.
-  * apply cgr_trans with ((x ! t) ˖ gpr_nil). apply cgr_trans with (g (x ! t)). apply cgr_refl. apply cgr_choice_nil_rev. apply cgr_par_nil_rev.
+- exists p. exists ⓪. exists ⓪. split ; try split.
+  * apply cgr_trans with ((x ! • p) + ⓪). apply cgr_trans with (x ! • p). apply cgr_refl. apply cgr_choice_nil_rev. apply cgr_par_nil_rev.
   * apply cgr_par_nil_rev.
   * reflexivity.
-- destruct (IHTransition x). reflexivity. decompose record H. exists x0. exists x1. exists (x2 ∥ q). split; try split.
-  * apply cgr_trans with ((((x ! x0) ˖ x1) ∥ x2) ∥ q). apply cgr_par. exact H0. apply cgr_par_assoc.
-  * apply cgr_trans with ((x0 ∥ x2) ∥ q). apply cgr_par. exact H1. apply cgr_par_assoc.
+- destruct (IHTransition x). reflexivity. decompose record H. exists x0. exists x1. exists (x2 ‖ q). split; try split.
+  * apply cgr_trans with ((((x ! • x0) + x1) ‖ x2) ‖ q). apply cgr_par. exact H0. apply cgr_par_assoc.
+  * apply cgr_trans with ((x0 ‖ x2) ‖ q). apply cgr_par. exact H1. apply cgr_par_assoc.
   * intros. inversion H2. inversion H4.
-- destruct (IHTransition x). reflexivity. decompose record H. exists x0. exists x1. exists (x2 ∥ p). split; try split.
-  * apply cgr_trans with ((((x ! x0) ˖ x1) ∥ x2) ∥ p). apply cgr_trans with (q1 ∥ p). apply cgr_par_com. apply cgr_par. exact H0. apply cgr_par_assoc.
-  * apply cgr_trans with ((x0 ∥ x2) ∥ p). apply cgr_trans with (q2 ∥ p). apply cgr_par_com. apply cgr_par. exact H1. apply cgr_par_assoc.
+- destruct (IHTransition x). reflexivity. decompose record H. exists x0. exists x1. exists (x2 ‖ p). split; try split.
+  * apply cgr_trans with ((((x ! • x0) + x1) ‖ x2) ‖ p). apply cgr_trans with (q1 ‖ p). apply cgr_par_com. apply cgr_par. exact H0. apply cgr_par_assoc.
+  * apply cgr_trans with ((x0 ‖ x2) ‖ p). apply cgr_trans with (q2 ‖ p). apply cgr_par_com. apply cgr_par. exact H1. apply cgr_par_assoc.
   * intros. inversion H2. inversion H4.
-- destruct (IHTransition x). reflexivity. decompose record H. exists x0. exists (gpr_choice x1 p2). exists θ. split ; try split.
-  * apply cgr_trans with ((x ! x0) ˖ gpr_choice x1 p2). apply cgr_trans with ((gpr_choice (x ! x0) x1) ˖ p2).
-    apply cgr_choice. assert (x2 = θ). apply H3. exists p1. reflexivity. rewrite H2 in H0. apply transitivity with (((x ! x0) ˖ x1) ∥ θ).
+- destruct (IHTransition x). reflexivity. decompose record H. exists x0. exists (x1 + p2). exists ⓪. split ; try split.
+  * apply cgr_trans with ((x ! • x0) + (x1 + p2)). apply cgr_trans with (((x ! • x0) + x1) + p2).
+    apply cgr_choice. assert (x2 = ⓪). apply H3. exists p1. reflexivity. rewrite H2 in H0. apply transitivity with (((x ! • x0) + x1) ‖ ⓪).
     exact H0. apply cgr_par_nil. apply cgr_choice_assoc. apply cgr_par_nil_rev.
-  * assert (x2 = θ). apply H3. exists p1. reflexivity. rewrite H2 in H1. exact H1.
+  * assert (x2 = ⓪). apply H3. exists p1. reflexivity. rewrite H2 in H1. exact H1.
   * reflexivity.
-- destruct (IHTransition x). reflexivity. decompose record H. exists x0. exists (gpr_choice x1 p1). exists θ. split; try split.
-  * apply cgr_trans with ((x ! x0) ˖ gpr_choice x1 p1). apply cgr_trans with ((gpr_choice (x ! x0) x1) ˖ p1).
-    apply cgr_trans with (p2 ˖ p1). apply cgr_choice_com. apply cgr_choice. assert (x2 = θ). apply H3. exists p2. reflexivity.
-    apply cgr_trans with (((x ! x0) ˖ x1) ∥ x2). exact H0. rewrite H2. apply cgr_par_nil. apply cgr_choice_assoc. apply cgr_par_nil_rev.
-  * assert (x2 = θ). apply H3. exists p2. reflexivity. rewrite <-H2. exact H1.
+- destruct (IHTransition x). reflexivity. decompose record H. exists x0. exists (x1 + p1). exists ⓪. split; try split.
+  * apply cgr_trans with ((x ! • x0) + (x1 + p1)). apply cgr_trans with (((x ! • x0) + x1) + p1).
+    apply cgr_trans with (p2 + p1). apply cgr_choice_com. apply cgr_choice. assert (x2 = ⓪). apply H3. exists p2. reflexivity.
+    apply cgr_trans with (((x ! • x0) + x1) ‖ x2). exact H0. rewrite H2. apply cgr_par_nil. apply cgr_choice_assoc. apply cgr_par_nil_rev.
+  * assert (x2 = ⓪). apply H3. exists p2. reflexivity. rewrite <-H2. exact H1.
   * reflexivity.
 Qed.
 
 (* For the (LTS-transition), the transitable Guards and transitted terms, that performs a Tau ,
 are pretty all the same, up to ≡* *)
 Lemma TransitionShapeForTauAndGuard : forall P V, ((lts P τ V) /\ (exists L, P = (g L))) -> 
-(exists Q M, ((P ≡* ((gpr_tau Q) ˖ M))) /\ (V ≡* (Q))).
+(exists Q M, ((P ≡* ((t • Q) + M))) /\ (V ≡* (Q))).
 Proof.
 intros P V Hyp. 
 destruct Hyp. rename H into Transition. dependent induction Transition.
-- exists t. exists gpr_nil. split. 
+- exists p. exists ⓪. split. 
   * apply cgr_choice_nil_rev.
   * apply cgr_refl.
 - inversion H0. inversion H.
@@ -519,10 +527,10 @@ destruct Hyp. rename H into Transition. dependent induction Transition.
 - inversion H0. inversion H.
 - inversion H0. inversion H.
 - destruct (IHTransition (reflexivity τ)). exists p1. reflexivity. destruct H. destruct H.  exists x. 
-  exists (gpr_choice x0 p2). split. apply cgr_trans with ((gpr_choice (gpr_tau x) x0) ˖ p2). apply cgr_choice. exact H.
+  exists (x0 + p2). split. apply cgr_trans with (((t • x) + x0) + p2). apply cgr_choice. exact H.
   apply cgr_choice_assoc. exact H1.
 - destruct (IHTransition (reflexivity τ)). exists p2. reflexivity. destruct H. destruct H.  exists x. 
-  exists (gpr_choice x0 p1). split. apply cgr_trans with ((gpr_choice (gpr_tau x) x0) ˖ p1). apply cgr_trans with (p2 ˖ p1). 
+  exists (x0 + p1). split. apply cgr_trans with (((t • x) + x0) + p1). apply cgr_trans with (p2 + p1). 
   apply cgr_choice_com. apply cgr_choice. exact H. apply cgr_choice_assoc. exact H1.
 Qed.
 
@@ -535,8 +543,8 @@ induction p as (p & Hp) using
     (well_founded_induction (wf_inverse_image _ nat _ size Nat.lt_wf_0)).
 destruct p.
   - simpl. intro. apply cgr_fullpar.
-    apply Hp. simpl. rewrite <-Nat.add_succ_r. apply PeanoNat.Nat.lt_add_pos_r. apply Nat.lt_0_succ. exact H. 
-    apply Hp. simpl. rewrite <-Nat.add_succ_l. apply PeanoNat.Nat.lt_add_pos_l. apply Nat.lt_0_succ. exact H.
+    apply Hp. simpl. auto with arith. assumption. 
+    apply Hp. simpl. auto with arith. assumption.
   - simpl. intro. destruct (decide (x = n)). exact H. reflexivity.
   - simpl. intro. destruct (decide (x = n)). reflexivity. apply cgr_recursion. apply Hp. simpl. auto. exact H.
   - destruct g0.
@@ -546,12 +554,8 @@ destruct p.
     * intro. apply cgr_output. apply Hp. simpl. auto. exact H.
     * intro. apply cgr_tau. apply Hp. simpl. auto. exact H.
     * intro. simpl. apply cgr_fullchoice. 
-      assert (pr_subst x (g g0_1) q ≡* pr_subst x (g g0_1) q'). apply Hp. simpl. 
-      rewrite <-Nat.add_succ_r. apply PeanoNat.Nat.lt_add_pos_r. apply Nat.lt_0_succ. exact H.
-      exact H0.
-      assert (pr_subst x (g g0_2) q ≡* pr_subst x (g g0_2) q'). apply Hp. simpl. 
-      rewrite <-Nat.add_succ_l. apply PeanoNat.Nat.lt_add_pos_l. apply Nat.lt_0_succ. exact H.
-      exact H0.
+      assert (pr_subst x (g g0_1) q ≡* pr_subst x (g g0_1) q'). apply Hp. simpl. auto with arith. assumption. assumption. 
+      assert (pr_subst x (g g0_2) q ≡* pr_subst x (g g0_2) q'). apply Hp. simpl. auto with arith. assumption. assumption.
 Qed.
 
 (* ≡ respects the substitution of his variable*)
@@ -575,11 +579,9 @@ Proof.
   - simpl. constructor. apply Hp. subst. simpl. auto. exact H.
   - simpl. constructor. apply Hp. subst. simpl. auto. exact H. 
   - simpl. constructor. apply Hp. subst. simpl. auto. exact H. 
-  - simpl. constructor. apply Hp. subst. simpl. rewrite <-Nat.add_succ_r. apply PeanoNat.Nat.lt_add_pos_r. apply Nat.lt_0_succ.
-    exact H.
+  - simpl. constructor. apply Hp. subst. simpl. auto with arith. assumption.
   - simpl. apply cgr_choice_step. 
-    assert (pr_subst n (g p1) q ≡ pr_subst n (g q1) q). apply Hp. subst. simpl. rewrite <-Nat.add_succ_r. apply PeanoNat.Nat.lt_add_pos_r. apply Nat.lt_0_succ.
-    exact H. exact H2.
+    assert (pr_subst n (g p1) q ≡ pr_subst n (g q1) q). apply Hp. subst. simpl. auto with arith. assumption. assumption.
 Qed.
 
 (* ≡* respects the substitution of his variable *)
@@ -614,52 +616,52 @@ Proof.
   - dependent induction H. 
 (* reasonning about all possible cases due to the structure of terms *)
     + intros. exists q.  split.  exact l. reflexivity. 
-    + intros. exists (q ∥ θ). split. apply lts_parL. exact l. auto with cgr (*par contexte parallele*). 
+    + intros. exists (q ‖ ⓪). split. apply lts_parL. exact l. auto with cgr (*par contexte parallele*). 
     + intros. dependent destruction l. inversion l2. inversion l1. exists p2. split. exact l. auto with cgr. 
       inversion l.
     + intros. dependent destruction l.
-      -- exists (q2 ∥ p2). split. eapply lts_comR. instantiate (1:= a). exact l1. exact l2. auto with cgr.
-      -- exists (p2 ∥ q2). split. eapply lts_comL. instantiate (1:= a). exact l1. exact l2. auto with cgr.
-      -- exists (p ∥ p2). split. apply lts_parR. exact l. auto with cgr.
-      -- exists (q2 ∥ q). split. apply lts_parL. exact l. auto with cgr.
+      -- exists (q2 ‖ p2). split. eapply lts_comR. instantiate (1:= a). exact l1. exact l2. auto with cgr.
+      -- exists (p2 ‖ q2). split. eapply lts_comL. instantiate (1:= a). exact l1. exact l2. auto with cgr.
+      -- exists (p ‖ p2). split. apply lts_parR. exact l. auto with cgr.
+      -- exists (q2 ‖ q). split. apply lts_parL. exact l. auto with cgr.
     + intros. dependent destruction l.
       -- dependent destruction l2. 
-         * exists ((p2 ∥ p0) ∥ r). split.
+         * exists ((p2 ‖ p0) ‖ r). split.
            apply lts_parL. eapply lts_comL. instantiate (1:= a). exact l1. exact l2. auto with cgr.
-         * exists ((p2 ∥ q) ∥ q2). split. eapply lts_comL. instantiate (1:= a). apply lts_parL. exact l1.
+         * exists ((p2 ‖ q) ‖ q2). split. eapply lts_comL. instantiate (1:= a). apply lts_parL. exact l1.
            exact l2. apply cgr_par_assoc.
       -- dependent destruction l1. 
-         * exists ((q2 ∥ p2) ∥ r). split. apply lts_parL. eapply lts_comR. instantiate (1:= a). exact l1.
+         * exists ((q2 ‖ p2) ‖ r). split. apply lts_parL. eapply lts_comR. instantiate (1:= a). exact l1.
            exact l2. auto with cgr.
-         * exists ((q2 ∥ q) ∥ q0). split. eapply lts_comR. instantiate (1:= a). exact l1. apply lts_parL.
+         * exists ((q2 ‖ q) ‖ q0). split. eapply lts_comR. instantiate (1:= a). exact l1. apply lts_parL.
            exact l2. auto with cgr.
-      -- exists ((p2 ∥ q) ∥ r). split. apply lts_parL. apply lts_parL. exact l. auto with cgr.
+      -- exists ((p2 ‖ q) ‖ r). split. apply lts_parL. apply lts_parL. exact l. auto with cgr.
       -- dependent destruction l.
-         * exists ((p ∥ p2) ∥ q2). split. eapply lts_comL. instantiate (1:= a). apply lts_parR. exact l1.
+         * exists ((p ‖ p2) ‖ q2). split. eapply lts_comL. instantiate (1:= a). apply lts_parR. exact l1.
            exact l2. auto with cgr.
-         * exists ((p ∥ q2) ∥ p2). split. eapply lts_comR. instantiate (1:= a). exact l1. apply lts_parR.
+         * exists ((p ‖ q2) ‖ p2). split. eapply lts_comR. instantiate (1:= a). exact l1. apply lts_parR.
            exact l2. auto with cgr.
-         * exists ((p ∥ p2) ∥ r). split. apply lts_parL. apply lts_parR. exact l. auto with cgr.
-         * exists ((p ∥ q) ∥ q2). split. apply lts_parR. exact l. auto with cgr.
+         * exists ((p ‖ p2) ‖ r). split. apply lts_parL. apply lts_parR. exact l. auto with cgr.
+         * exists ((p ‖ q) ‖ q2). split. apply lts_parR. exact l. auto with cgr.
     + intros. dependent destruction l.
       -- dependent destruction l1. 
-         * exists (p2 ∥ (q ∥ q2)). split.
+         * exists (p2 ‖ (q ‖ q2)). split.
            eapply lts_comL. instantiate (1:= a). exact l1. apply lts_parR. exact l2. auto with cgr.
-         * exists (p ∥ (q0 ∥ q2)). split. apply lts_parR. eapply lts_comL. instantiate (1:= a). exact l1.
+         * exists (p ‖ (q0 ‖ q2)). split. apply lts_parR. eapply lts_comL. instantiate (1:= a). exact l1.
            exact l2. auto with cgr.
       -- dependent destruction l2. 
-         * exists (p0 ∥ (q ∥ p2)). split. eapply lts_comR. instantiate (1:= a). apply lts_parR.  exact l1.
+         * exists (p0 ‖ (q ‖ p2)). split. eapply lts_comR. instantiate (1:= a). apply lts_parR.  exact l1.
            exact l2. auto with cgr.
-         * exists (p ∥ (q2 ∥ p2)). split. apply lts_parR. eapply lts_comR. instantiate (1:= a). exact l1. 
+         * exists (p ‖ (q2 ‖ p2)). split. apply lts_parR. eapply lts_comR. instantiate (1:= a). exact l1. 
            exact l2. auto with cgr.
       -- dependent destruction l.
-         * exists (p2 ∥ (q2 ∥ r)). split. eapply lts_comL. instantiate (1:= a).  exact l1. apply lts_parL.
+         * exists (p2 ‖ (q2 ‖ r)). split. eapply lts_comL. instantiate (1:= a).  exact l1. apply lts_parL.
            exact l2. auto with cgr.
-         * exists (q2 ∥ (p2 ∥ r)). split. eapply lts_comR. instantiate (1:= a). apply lts_parL. exact l1. 
+         * exists (q2 ‖ (p2 ‖ r)). split. eapply lts_comR. instantiate (1:= a). apply lts_parL. exact l1. 
            exact l2. auto with cgr.
-         * exists (p2 ∥( q ∥ r)). split. apply lts_parL. exact l. auto with cgr.
-         * exists (p ∥ (q2 ∥ r)). split. apply lts_parR. apply lts_parL. exact l. auto with cgr.
-      -- exists (p ∥ (q ∥ q2)). split. apply lts_parR. apply lts_parR. exact l. auto with cgr.
+         * exists (p2 ‖( q ‖ r)). split. apply lts_parL. exact l. auto with cgr.
+         * exists (p ‖ (q2 ‖ r)). split. apply lts_parR. apply lts_parL. exact l. auto with cgr.
+      -- exists (p ‖ (q ‖ q2)). split. apply lts_parR. apply lts_parR. exact l. auto with cgr.
     + intros. exists q.  split. apply lts_choiceL.  exact l. auto with cgr.
     + intros. dependent destruction l.
       -- exists q. split. exact l. auto with cgr.
@@ -683,12 +685,12 @@ Proof.
     + intros. dependent destruction l. exists p. split. apply lts_input. constructor. apply H.
     + intros. dependent destruction l. exists p. split. apply lts_output. constructor. apply H.
     + intros. dependent destruction l. 
-      -- destruct (IHcgr_step p2 (ActExt (ActOut a))). exact l1. exists (x ∥ q2). split. eapply lts_comL. destruct H0. exact l.
+      -- destruct (IHcgr_step p2 (ActExt (ActOut a))). exact l1. exists (x ‖ q2). split. eapply lts_comL. destruct H0. exact l.
          exact l2. destruct H0. auto with cgr.
-      -- destruct (IHcgr_step q2 (ActExt (ActIn a))). exact l2. exists (x ∥ p2). split. eapply lts_comR. destruct H0. exact l1.
+      -- destruct (IHcgr_step q2 (ActExt (ActIn a))). exact l2. exists (x ‖ p2). split. eapply lts_comR. destruct H0. exact l1.
          destruct H0.  exact H0. destruct H0. auto with cgr.
-      -- destruct (IHcgr_step p2 α). exact l. destruct H0. exists (x ∥ r). split. apply lts_parL. exact H0. auto with cgr.
-      -- exists (p ∥ q2). split. apply lts_parR. exact l. apply cgr_par. constructor. exact H.
+      -- destruct (IHcgr_step p2 α). exact l. destruct H0. exists (x ‖ r). split. apply lts_parL. exact H0. auto with cgr.
+      -- exists (p ‖ q2). split. apply lts_parR. exact l. apply cgr_par. constructor. exact H.
     + intros. dependent destruction l.
       -- destruct (IHcgr_step q α). exact l. destruct H0. exists x. split. apply lts_choiceL. exact H0. exact H1.
       -- exists q. split. apply lts_choiceR. exact l. auto with cgr.
@@ -700,32 +702,33 @@ Qed.
 Lemma Reduction_Implies_TausAndCong : forall P Q, (sts P Q) -> (lts_sc P τ Q).
 Proof.
 intros P Q Reduction. 
-assert (((exists x P1 P2 M1 M2 S, ((P ≡* (((x!P1) ˖ M1) ∥ ((x ? P2) ˖ M2)) ∥ S)) /\ (Q ≡* ((P1 ∥ P2) ∥ S)))
-\/ (exists P1 M1 S, (P ≡* (((gpr_tau P1) ˖ M1) ∥ S)) /\ (Q ≡* (P1 ∥ S)))
-\/ (exists n P1 S, (P ≡* ((pr_rec n P1) ∥ S)) /\ (Q ≡* (pr_subst n P1 (pr_rec n P1) ∥ S))))). apply ReductionShape. exact Reduction. destruct H.
+assert (((exists x P1 P2 M1 M2 S, ((P ≡* (((x ! • P1) + M1) ‖ ((x ? • P2) + M2)) ‖ S)) /\ (Q ≡* ((P1 ‖ P2) ‖ S)))
+\/ (exists P1 M1 S, (P ≡* (((t • P1) + M1) ‖ S)) /\ (Q ≡* (P1 ‖ S)))
+\/ (exists n P1 S, (P ≡* ((rec n • P1) ‖ S)) /\ (Q ≡* (pr_subst n P1 (rec n • P1) ‖ S))))). 
+apply ReductionShape. exact Reduction. destruct H.
 
 (*First case τ by communication *)
 
-- decompose record H. assert (lts ((((x ! x0) ˖ x2) ∥ ((x ? x1) ˖ x3)) ∥ x4) τ ((x0 ∥ x1) ∥ x4)).
+- decompose record H. assert (lts ((((x ! • x0) + x2) ‖ ((x ? • x1) + x3)) ‖ x4) τ ((x0 ‖ x1) ‖ x4)).
   * apply lts_parL. eapply lts_comL. apply lts_choiceL. instantiate (1:= x). apply lts_output. apply lts_choiceL. apply lts_input.
-  * assert (lts_sc1 P τ ((x0 ∥ x1) ∥ x4)). exists ((((x ! x0) ˖ x2) ∥ ((x ? x1) ˖ x3)) ∥ x4). split. exact H0. exact H1.
-    assert (lts_sc P τ ((x0 ∥ x1) ∥ x4)). apply Congruence_Respects_Transition. exact H3. destruct H4. destruct H4. 
-    exists x5. split. exact H4. apply transitivity with ((x0 ∥ x1) ∥ x4). exact H5. symmetry. exact H2.
+  * assert (lts_sc1 P τ ((x0 ‖ x1) ‖ x4)). exists ((((x ! • x0) + x2) ‖ ((x ? • x1) + x3)) ‖ x4). split. exact H0. exact H1.
+    assert (lts_sc P τ ((x0 ‖ x1) ‖ x4)). apply Congruence_Respects_Transition. exact H3. destruct H4. destruct H4. 
+    exists x5. split. exact H4. apply transitivity with ((x0 ‖ x1) ‖ x4). exact H5. symmetry. exact H2.
 
 - destruct H. 
 
 (*Second case τ by Tau Action *)
 
-  * decompose record H. assert (lts ((gpr_tau x ˖ x0) ∥ x1) τ (x ∥ x1)). constructor. apply lts_choiceL. apply lts_tau.  
-    assert (lts_sc1 P τ (x ∥ x1)). exists ((gpr_tau x ˖ x0) ∥ x1). split. exact H1. exact H0.
-    assert (lts_sc P τ (x ∥ x1)). apply Congruence_Respects_Transition. exact H3. destruct H4. destruct H4. 
-    exists x2. split. exact H4. apply transitivity with (x ∥ x1). exact H5. symmetry. exact H2.
+  * decompose record H. assert (lts ((t • x + x0) ‖ x1) τ (x ‖ x1)). constructor. apply lts_choiceL. apply lts_tau.  
+    assert (lts_sc1 P τ (x ‖ x1)). exists ((t • x + x0) ‖ x1). split. exact H1. exact H0.
+    assert (lts_sc P τ (x ‖ x1)). apply Congruence_Respects_Transition. exact H3. destruct H4. destruct H4. 
+    exists x2. split. exact H4. apply transitivity with (x ‖ x1). exact H5. symmetry. exact H2.
 
 (*Third case τ by rec *)
-  * decompose record H. assert (lts (pr_rec x x0 ∥ x1) τ (pr_subst x x0 (pr_rec x x0) ∥ x1)). constructor. apply lts_rec.  
-    assert (lts_sc1 P τ ((pr_subst x x0 (pr_rec x x0) ∥ x1))). exists (pr_rec x x0 ∥ x1). split. exact H1. exact H0.
-    assert (lts_sc P τ (pr_subst x x0 (pr_rec x x0) ∥ x1)). apply Congruence_Respects_Transition. exact H3. destruct H4. destruct H4. 
-    exists x2. split. exact H4. apply transitivity with (pr_subst x x0 (pr_rec x x0) ∥ x1). exact H5. symmetry. exact H2.
+  * decompose record H. assert (lts (rec x • x0 ‖ x1) τ (pr_subst x x0 (rec x • x0) ‖ x1)). constructor. apply lts_rec.  
+    assert (lts_sc1 P τ ((pr_subst x x0 (rec x • x0) ‖ x1))). exists (rec x • x0 ‖ x1). split. exact H1. exact H0.
+    assert (lts_sc P τ (pr_subst x x0 (rec x • x0) ‖ x1)). apply Congruence_Respects_Transition. exact H3. destruct H4. destruct H4. 
+    exists x2. split. exact H4. apply transitivity with (pr_subst x x0 (rec x • x0) ‖ x1). exact H5. symmetry. exact H2.
 Qed.
 
 
@@ -737,34 +740,34 @@ exact H1.
 Qed.
 
 (* Some lemmas for multiple parallele processes to simplify the statements of proof*)
-Lemma InversionParallele : forall P Q R S, (P ∥ Q) ∥ (R ∥ S) ≡* (P ∥ R) ∥ (Q ∥ S) .
+Lemma InversionParallele : forall P Q R S, (P ‖ Q) ‖ (R ‖ S) ≡* (P ‖ R) ‖ (Q ‖ S) .
 Proof.
 intros.
-apply transitivity with (((P ∥ Q) ∥ R) ∥ S). apply cgr_par_assoc_rev.
-apply transitivity with ((P ∥ (Q ∥ R)) ∥ S). apply cgr_par. apply cgr_par_assoc.
-apply transitivity with (((Q ∥ R) ∥ P) ∥ S). apply cgr_par. apply cgr_par_com.
-apply transitivity with ((Q ∥ R) ∥ (P ∥ S)). apply cgr_par_assoc.
-apply transitivity with ((R ∥ Q) ∥ (P ∥ S)). apply cgr_par. apply cgr_par_com.
-apply transitivity with (((R ∥ Q) ∥ P) ∥ S). apply cgr_par_assoc_rev.
-apply transitivity with ((P ∥ (R ∥ Q)) ∥ S). apply cgr_par. apply cgr_par_com.
-apply transitivity with (((P ∥ R) ∥ Q) ∥ S). apply cgr_par. apply cgr_par_assoc_rev.
-apply transitivity with ((P ∥ R) ∥ (Q ∥ S)). apply cgr_par_assoc.
+apply transitivity with (((P ‖ Q) ‖ R) ‖ S). apply cgr_par_assoc_rev.
+apply transitivity with ((P ‖ (Q ‖ R)) ‖ S). apply cgr_par. apply cgr_par_assoc.
+apply transitivity with (((Q ‖ R) ‖ P) ‖ S). apply cgr_par. apply cgr_par_com.
+apply transitivity with ((Q ‖ R) ‖ (P ‖ S)). apply cgr_par_assoc.
+apply transitivity with ((R ‖ Q) ‖ (P ‖ S)). apply cgr_par. apply cgr_par_com.
+apply transitivity with (((R ‖ Q) ‖ P) ‖ S). apply cgr_par_assoc_rev.
+apply transitivity with ((P ‖ (R ‖ Q)) ‖ S). apply cgr_par. apply cgr_par_com.
+apply transitivity with (((P ‖ R) ‖ Q) ‖ S). apply cgr_par. apply cgr_par_assoc_rev.
+apply transitivity with ((P ‖ R) ‖ (Q ‖ S)). apply cgr_par_assoc.
 reflexivity.
 Qed.
-Lemma InversionParallele2 : forall P Q R S, (P ∥ Q) ∥ (R ∥ S) ≡* (R ∥ P) ∥ (S ∥ Q).
+Lemma InversionParallele2 : forall P Q R S, (P ‖ Q) ‖ (R ‖ S) ≡* (R ‖ P) ‖ (S ‖ Q).
 Proof.
 intros. 
-apply transitivity with ((P ∥ R) ∥ (Q ∥ S)). apply InversionParallele.
-apply transitivity with ((R ∥ P) ∥ (Q ∥ S)). apply cgr_par. apply cgr_par_com.
-apply transitivity with ((Q ∥ S) ∥ (R ∥ P)). apply cgr_par_com.
-apply transitivity with ((S ∥ Q) ∥ (R ∥ P)). apply cgr_par. apply cgr_par_com.
+apply transitivity with ((P ‖ R) ‖ (Q ‖ S)). apply InversionParallele.
+apply transitivity with ((R ‖ P) ‖ (Q ‖ S)). apply cgr_par. apply cgr_par_com.
+apply transitivity with ((Q ‖ S) ‖ (R ‖ P)). apply cgr_par_com.
+apply transitivity with ((S ‖ Q) ‖ (R ‖ P)). apply cgr_par. apply cgr_par_com.
 apply cgr_par_com.
 Qed.
-Lemma InversionParallele3 : forall P Q R S, (P ∥ Q) ∥ (R ∥ S) ≡* (R ∥ Q) ∥ (P ∥ S).
+Lemma InversionParallele3 : forall P Q R S, (P ‖ Q) ‖ (R ‖ S) ≡* (R ‖ Q) ‖ (P ‖ S).
 Proof.
 intros.
-apply transitivity with ((Q ∥ P) ∥ (R ∥ S)). apply cgr_par. apply cgr_par_com.
-apply transitivity with ((Q ∥ R) ∥ (P ∥ S)). apply InversionParallele. apply cgr_par. apply cgr_par_com.
+apply transitivity with ((Q ‖ P) ‖ (R ‖ S)). apply cgr_par. apply cgr_par_com.
+apply transitivity with ((Q ‖ R) ‖ (P ‖ S)). apply InversionParallele. apply cgr_par. apply cgr_par_com.
 Qed.
 
 
@@ -772,36 +775,36 @@ Lemma Taus_Implies_Reduction : forall P Q, (lts P τ Q) -> (sts P Q).
 Proof.
 intros.
 dependent induction H.
-  - eapply sts_cong.  instantiate (1:=  ((gpr_tau t) ˖ gpr_nil)). apply cgr_choice_nil_rev. instantiate (1:=t).
+  - eapply sts_cong. instantiate (1:=  ((t • p) + ⓪)). apply cgr_choice_nil_rev. instantiate (1:=p).
     apply sts_tau. apply cgr_refl.
   - apply sts_rec.
   - destruct (TransitionShapeForOutput p1 p2 a). exact H. destruct H1. destruct H1. destruct H1. destruct H2.
     destruct (TransitionShapeForInput q1 q2 a). exact H0. destruct H4. destruct H4. destruct H4. destruct H5.
-    eapply sts_cong. instantiate (1:=(((a ! x) ˖ x0) ∥ ((a ? x2) ˖ x3)) ∥ (x1 ∥ x4)).
-    apply cgr_trans with ((((a ! x) ˖ x0) ∥ x1) ∥ (((a ? x2) ˖ x3) ∥ x4)). apply cgr_fullpar. exact H1. exact H4.
+    eapply sts_cong. instantiate (1:=(((a ! • x) + x0) ‖ ((a ? • x2) + x3)) ‖ (x1 ‖ x4)).
+    apply cgr_trans with ((((a ! • x) + x0) ‖ x1) ‖ (((a ? • x2) + x3) ‖ x4)). apply cgr_fullpar. exact H1. exact H4.
     apply InversionParallele. 
-    instantiate (1 := (x ∥ x2) ∥ (x1 ∥ x4)). apply sts_par. apply sts_com.
-    apply transitivity with ((x ∥ x1) ∥ (x2 ∥ x4)). apply InversionParallele. apply cgr_fullpar. 
+    instantiate (1 := (x ‖ x2) ‖ (x1 ‖ x4)). apply sts_par. apply sts_com.
+    apply transitivity with ((x ‖ x1) ‖ (x2 ‖ x4)). apply InversionParallele. apply cgr_fullpar. 
     symmetry. exact H2. symmetry. exact H5.
   - destruct (TransitionShapeForOutput p1 p2 a). exact H. destruct H1. destruct H1. destruct H1. destruct H2.
     destruct (TransitionShapeForInput q1 q2 a). exact H0. destruct H4. destruct H4. destruct H4. destruct H5.
-    eapply sts_cong. instantiate (1:=(((a ! x) ˖ x0) ∥ ((a ? x2) ˖ x3)) ∥ (x1 ∥ x4)).
-    apply transitivity with (p1 ∥ q1). apply cgr_par_com.
-    apply transitivity with ((((a ! x) ˖ x0) ∥ x1) ∥ (((a ? x2) ˖ x3) ∥ x4)).
+    eapply sts_cong. instantiate (1:=(((a ! • x) + x0) ‖ ((a ? • x2) + x3)) ‖ (x1 ‖ x4)).
+    apply transitivity with (p1 ‖ q1). apply cgr_par_com.
+    apply transitivity with ((((a ! • x) + x0) ‖ x1) ‖ (((a ? • x2) + x3) ‖ x4)).
     apply cgr_fullpar. exact H1. exact H4. apply InversionParallele. 
-    instantiate (1 := (x ∥ x2) ∥ (x1 ∥ x4)). apply sts_par. apply sts_com.
-    apply transitivity with ((x ∥ x1) ∥ (x2 ∥ x4)). apply InversionParallele. apply transitivity with (p2 ∥ q2). apply cgr_fullpar. 
+    instantiate (1 := (x ‖ x2) ‖ (x1 ‖ x4)). apply sts_par. apply sts_com.
+    apply transitivity with ((x ‖ x1) ‖ (x2 ‖ x4)). apply InversionParallele. apply transitivity with (p2 ‖ q2). apply cgr_fullpar. 
     symmetry. exact H2. symmetry. exact H5. apply cgr_par_com.
 - apply sts_par. apply IHlts. reflexivity.
-- eapply sts_cong. instantiate (1:= q1 ∥ p). apply cgr_par_com. instantiate (1:= q2 ∥ p).
+- eapply sts_cong. instantiate (1:= q1 ‖ p). apply cgr_par_com. instantiate (1:= q2 ‖ p).
   apply sts_par. apply IHlts. reflexivity. apply cgr_par_com.
 - destruct (TransitionShapeForTauAndGuard (g p1) q). split. exact H. exists p1. reflexivity.
-  destruct H0. destruct H0. eapply sts_cong. instantiate (1:= (((gpr_tau x) ˖ (gpr_choice x0  p2)))).
-  apply transitivity with ((gpr_choice (gpr_tau x) x0 ) ˖ p2). apply cgr_choice. exact H0. apply cgr_choice_assoc.
+  destruct H0. destruct H0. eapply sts_cong. instantiate (1:= (((t • x) + (x0 + p2)))).
+  apply transitivity with (g (((t • x) + x0 ) + p2)). apply cgr_choice. exact H0. apply cgr_choice_assoc.
   instantiate (1:= x). apply sts_tau. symmetry. exact H1.
 - destruct (TransitionShapeForTauAndGuard (g p2) q). split. exact H. exists p2. reflexivity.
-  destruct H0. destruct H0. eapply sts_cong. instantiate (1:= (((gpr_tau x) ˖ (gpr_choice x0  p1)))).
-  apply transitivity with ((gpr_choice (gpr_tau x) x0 ) ˖ p1). apply transitivity with (p2 ˖ p1). apply cgr_choice_com.
+  destruct H0. destruct H0. eapply sts_cong. instantiate (1:= (((t • x) + (x0 + p1)))).
+  apply transitivity with (g (((t • x) + x0 ) + p1)). apply transitivity with (g (p2 + p1)). apply cgr_choice_com.
   apply cgr_choice. exact H0. apply cgr_choice_assoc. instantiate (1:= x). apply sts_tau. symmetry. exact H1.
 Qed.
 
@@ -818,8 +821,3 @@ intros. split.
 * apply TausAndCong_Implies_Reduction.
 * apply Reduction_Implies_TausAndCong.
 Qed.
-
-
-
-
-
